theories/L/Datatypes/LLists.v
@@ -2,6 +2,8 @@ From Undecidability.L.Tactics Require Import LTactics GenEncode.
 From Undecidability.L.Datatypes Require Import LBool LOptions LProd LLNat.
 Require Export List PslBase.Lists.Filter Datatypes.
 Require Undecidability.L.Datatypes.Lists. 
+From Undecidability.L Require Import Functions.EqBool.
+
 
 (** ** Encoding of lists *)
 
@@ -195,49 +197,6 @@ Section list_eqb.
   Qed.
 
 End list_eqb.
-Section int.
-
-  Context {X : Type}.
-  Context {HX : registered X}.
-
-  Fixpoint list_eqbTime (eqbT: timeComplexity (X -> X -> bool)) (A B:list X) :=
-    match A,B with
-      a::A,b::B => callTime2 eqbT a b + 22 + list_eqbTime eqbT A B
-    | _,_ => 9
-    end.
-  
-  Global Instance term_list_eqb : computableTime' (list_eqb (X:=X))
-                                                   (fun _ eqbT => (1,(fun A _ => (5,fun B _ => (list_eqbTime eqbT A B,tt))))).
-  Proof.
-    extract.
-    solverec.                                                                                             
-  Defined.
-
-  Definition list_eqbTime_leq (eqbT: timeComplexity (X -> X -> bool)) (A B:list X) k:
-    (forall a b, callTime2 eqbT a b <= k)
-    -> list_eqbTime eqbT A B <= length A * (k+22) + 9.
-  Proof.
-    intros H'. induction A in B|-*.
-    -cbn. omega.
-    -destruct B.
-     {cbn. intuition. }
-     cbn - [callTime2]. setoid_rewrite IHA.
-     rewrite H'. ring_simplify. intuition.
-  Qed.
-
-  
-  Lemma list_eqbTime_bound_r (eqbT : timeComplexity (X -> X -> bool)) (A B : list X) f:
-    (forall (x y:X), callTime2 eqbT x y <= f y) ->
-    list_eqbTime eqbT A B <= sumn (map f B) + 9 + length B * 22.
-  Proof.
-    intros H.
-    induction A in B|-*;unfold list_eqbTime;fold list_eqbTime. now Lia.lia.
-    destruct B.
-    -cbn. Lia.lia.
-    -rewrite H,IHA. cbn [length map sumn]. Lia.lia.
-  Qed.
-  
-End int.
 
 Section list_prod.
 
